ArchSem/ListSet.lean
@@ -1,0 +1,309 @@
+import Std.Data.ExtTreeSet
+
+/-!
+This file implements a finite set type (similar to MathLib's FinSet) as a
+Quotient type over lists. This is primarily used for representing the set of
+states & results in the non-deterministic monad. Using a ListSet for this role
+means that we can effectivly choose when deduplication happens: if we were
+using a hash set for example, then we would be forced to hash every state after
+every monadic bind which could be costly.
+
+De-duplication is done with the `prune` function.
+TODO: implement an optimized deduplication of elements using a user-supplied
+      hash function.
+-/
+
+namespace ArchSem
+
+/-- The quotient relation for ListSets: lists that contain the same elements. -/
+def ListSet.r {α : Type} (a b : List α) : Prop :=
+  ∀ x : α, x ∈ a ↔ x ∈ b
+
+def ListSetSetoid (α : Type) : Setoid (List α) where
+  r := ListSet.r
+  iseqv := {
+    refl := by
+      simp [ListSet.r]
+    symm := by
+      simp only [ListSet.r]
+      intro l₁ l₂ h
+      simp [h]
+    trans := by
+      simp only [ListSet.r]
+      intro l₁ l₂ l₃ h₁ h₂ x
+      exact Iff.trans (h₁ x) (h₂ x)
+  }
+
+/--
+A finite set type implemented as a list up to the elements it contains.
+-/
+def ListSet (α : Type) := Quotient (ListSetSetoid α)
+
+def ListSet.empty : ListSet α := Quotient.mk (ListSetSetoid α) []
+
+def ListSet.ofList (l : List α) : ListSet α := Quotient.mk (ListSetSetoid α) l
+
+instance [DecidableEq α] : DecidableEq (ListSet α) := by
+  intro a b
+  refine Quotient.recOnSubsingleton₂ a b ?_
+  intro la lb
+  let p : Prop := la ⊆ lb ∧ lb ⊆ la
+  have hp : p ↔ ListSet.r la lb := by
+    constructor
+    · intro h x
+      constructor
+      · intro hx
+        exact h.1 hx
+      · intro hx
+        exact h.2 hx
+    · intro h
+      constructor
+      · intro x hx
+        exact (h x).mp hx
+      · intro x hx
+        exact (h x).mpr hx
+  by_cases h : p
+  · exact isTrue (Quotient.sound (hp.mp h))
+  · exact isFalse (fun heq => h (hp.mpr (Quotient.exact heq)))
+
+/--
+Deduplicate the internal elements of the ListSet.
+This has no logically observable effect (as proven by ListSet.prune_eq),
+but it can improve performance depending on your usecase.
+-/
+def ListSet.prune (l : ListSet α) [DecidableEq α] : ListSet α :=
+  Quotient.lift (fun l => ListSet.ofList l.eraseDups) (by
+    intro a b h
+    apply Quotient.sound
+    intro x
+    simpa [List.mem_eraseDups] using h x) l
+
+/--
+Prove that internal-deduplication has no observable effect.
+-/
+theorem ListSet.prune_eq {l : ListSet α} [DecidableEq α] : l.prune = l :=
+  Quotient.inductionOn l (by
+    intro l
+    apply Quotient.sound
+    intro x
+    simp [List.mem_eraseDups])
+
+/-- Set membership. -/
+def ListSet.mem (x : α) : ListSet α → Prop :=
+  Quotient.lift (fun l => x ∈ l) (by
+    intro a b h
+    exact propext (h x))
+
+instance : Membership α (ListSet α) where
+  mem s x := ListSet.mem x s
+
+-- Many of the ListSet lemmas have direct analogous in List.
+
+@[simp]
+theorem ListSet.mem_of_list {x : α} {l : List α}
+    : x ∈ ListSet.ofList l ↔ x ∈ l := by
+  change x ∈ l ↔ x ∈ l
+  simp
+
+theorem ListSet.not_mem_empty (x : α) : x ∉ ListSet.empty := by
+  change x ∉ ([] : List α)
+  simp
+
+theorem ListSet.ext {a b : ListSet α} (h : ∀ x, x ∈ a ↔ x ∈ b) : a = b := by
+  refine Quotient.inductionOn₂ a b ?_ h
+  intro la lb h
+  apply Quotient.sound
+  intro x
+  exact h x
+
+def ListSet.isEmpty : ListSet α → Bool :=
+  Quotient.lift List.isEmpty (by
+    intro a b
+    intro h
+    change ListSet.r a b at h
+    rw [ListSet.r] at h
+    cases a with
+    | nil =>
+      simp only [List.not_mem_nil, false_iff] at h
+      simp [List.eq_nil_iff_forall_not_mem.mpr h]
+    | cons head _ =>
+      specialize h head
+      simp only [List.mem_cons, true_or, true_iff] at h
+      simp [List.ne_nil_of_mem h]
+  )
+
+def ListSet.any (p : α → Bool) : ListSet α → Bool :=
+  Quotient.lift (fun a => a.any p) (by
+    intro a b h
+    apply Bool.eq_iff_iff.mpr
+    simp only [List.any_eq_true]
+    constructor
+    · rintro ⟨x, hx, hp⟩
+      exact ⟨x, (h x).mp hx, hp⟩
+    · rintro ⟨x, hx, hp⟩
+      exact ⟨x, (h x).mpr hx, hp⟩)
+
+theorem ListSet.any_eq_true {p : α → Bool} {s : ListSet α} :
+    s.any p = true ↔ ∃ x, x ∈ s ∧ p x = true := by
+  refine Quotient.inductionOn s ?_
+  intro l
+  change l.any p = true ↔ ∃ x, x ∈ l ∧ p x = true
+  simp only [List.any_eq_true]
+
+theorem ListSet.any_eq_false {p : α → Bool} {s : ListSet α} :
+    s.any p = false ↔ ∀ x, x ∈ s → p x = false := by
+  refine Quotient.inductionOn s ?_
+  intro l
+  change l.any p = false ↔ ∀ x, x ∈ l → p x = false
+  rw [List.any_eq_false]
+  constructor
+  · intro h x hx
+    specialize h x hx
+    cases hp : p x <;> simp [hp] at h ⊢
+  · intro h x hx
+    rw [h x hx]
+    simp
+
+/--
+Take the union of two list sets. Internally implemented as a list append
+with no-deduplication.
+-/
+def ListSet.union : ListSet α → ListSet α → ListSet α :=
+  Quotient.lift₂ (fun a b => ListSet.ofList (a ++ b)) (by
+    intro a₁ a₂ b₁ b₂ ha hb
+    apply Quotient.sound
+    intro x
+    simp only [List.mem_append]
+    constructor
+    · rintro (h | h)
+      · exact Or.inl ((ha x).mp h)
+      · exact Or.inr ((hb x).mp h)
+    · rintro (h | h)
+      · exact Or.inl ((ha x).mpr h)
+      · exact Or.inr ((hb x).mpr h))
+
+/--
+Map set elements. Internally implemented as a List map with no deduplication.
+-/
+def ListSet.map (f : α → β) : ListSet α → ListSet β :=
+  Quotient.lift (fun a => ListSet.ofList (a.map f)) (by
+    intro a b h
+    apply Quotient.sound
+    intro y
+    simp only [List.mem_map]
+    constructor
+    · rintro ⟨x, hx, rfl⟩
+      exact ⟨x, (h x).mp hx, rfl⟩
+    · rintro ⟨x, hx, rfl⟩
+      exact ⟨x, (h x).mpr hx, rfl⟩)
+
+/--
+Filter map set elements. Internally implemented as a List filtermap with no
+deduplication.
+-/
+def ListSet.filterMap (f : α → Option β) : ListSet α → ListSet β :=
+  Quotient.lift (fun a => ListSet.ofList (a.filterMap f)) (by
+    intro a b h
+    apply Quotient.sound
+    intro y
+    simp only [List.mem_filterMap]
+    constructor
+    · rintro ⟨x, hx, hf⟩
+      exact ⟨x, (h x).mp hx, hf⟩
+    · rintro ⟨x, hx, hf⟩
+      exact ⟨x, (h x).mpr hx, hf⟩)
+
+theorem ListSet.map_congr_left {l : ListSet α} {f g : α → β} (h : ∀ x ∈ l, f x = g x)
+    : ListSet.map f l = ListSet.map g l := by
+  revert h
+  refine Quotient.inductionOn l ?_
+  intro ls h
+  apply ListSet.ext
+  intro x
+  change x ∈ ls.map f ↔ x ∈ ls.map g
+  change ∀ x, x ∈ ls → f x = g x at h
+  simp only [List.mem_map]
+  apply Iff.intro
+  · rintro ⟨a, ha, hf⟩
+    refine ⟨a, ha, ?_⟩
+    rw [← h a ha]
+    exact hf
+  · rintro ⟨a, ha, hg⟩
+    refine ⟨a, ha, ?_⟩
+    rw [h a ha]
+    exact hg
+
+theorem ListSet.mem_map {x : β} {a : ListSet α} {f : α → β} :
+    x ∈ a.map f ↔ ∃ y, y ∈ a ∧ f y = x := by
+  simp only [ListSet.map]
+  refine Quotient.inductionOn a ?_
+  intro a
+  change x ∈ List.map f a ↔ ∃ y, y ∈ a ∧ f y = x
+  simp [List.mem_map]
+
+theorem ListSet.mem_union (x : α) (a b : ListSet α) :
+    x ∈ ListSet.union a b ↔ x ∈ a ∨ x ∈ b := by
+  refine Quotient.inductionOn₂ a b ?_
+  intro la lb
+  change ListSet.mem x (ListSet.ofList (la ++ lb)) ↔
+    ListSet.mem x (ListSet.ofList la) ∨ ListSet.mem x (ListSet.ofList lb)
+  simp [ListSet.mem, ListSet.ofList, Quotient.lift, Quotient.mk, List.mem_append]
+
+theorem ListSet.mem_foldr_union (x : α) (sets : List (ListSet α)) :
+    x ∈ sets.foldr ListSet.union (ListSet.ofList []) ↔ ∃ s, s ∈ sets ∧ x ∈ s := by
+  induction sets with
+  | nil =>
+    change ListSet.mem x (ListSet.ofList ([] : List α)) ↔ ∃ s, s ∈ [] ∧ x ∈ s
+    simp [ListSet.mem, ListSet.ofList, Quotient.lift, Quotient.mk]
+  | cons s sets ih =>
+    simp [List.foldr, ListSet.mem_union, ih, or_and_right, exists_or]
+
+/--
+Flatten the elements of a nested ListSet. This does no internal deduplication
+so consider running ListSet.prune afterwards.
+-/
+def ListSet.flatten : ListSet (ListSet α) → ListSet α :=
+  Quotient.lift (fun sets => sets.foldr ListSet.union ListSet.empty) (by
+    intro a b h
+    apply ListSet.ext
+    intro x
+    constructor
+    · intro hx
+      obtain ⟨s, hs, hxs⟩ := (ListSet.mem_foldr_union x a).mp hx
+      exact (ListSet.mem_foldr_union x b).mpr ⟨s, (h s).mp hs, hxs⟩
+    · intro hx
+      obtain ⟨s, hs, hxs⟩ := (ListSet.mem_foldr_union x b).mp hx
+      exact (ListSet.mem_foldr_union x a).mpr ⟨s, (h s).mpr hs, hxs⟩)
+
+def ListSet.mem_flatten (x : α) (a : ListSet (ListSet α)) :
+    x ∈ a.flatten ↔ ∃ b, b ∈ a ∧ x ∈ b := by
+  refine Quotient.inductionOn a ?_
+  intro as
+  induction as with
+  | nil =>
+    simp only [flatten]
+    change x ∈ [] ↔ ∃ b, b ∈ [] ∧ x ∈ b
+    simp
+  | cons h t ih =>
+    simp only [flatten] at ⊢ ih
+    change x ∈ List.foldr union empty (h::t) ↔ ∃ b, b ∈ (h::t) ∧ x ∈ b
+    change x ∈ List.foldr union empty t ↔ ∃ b, b ∈ t ∧ x ∈ b at ih
+    simp [ListSet.mem_union, ih]
+
+/--
+Extract the elements of a ListSet to a deduplicated and sorted list.
+We must specify a normalized order so that all equal ListSet's output
+the same list from this function.
+-/
+def ListSet.toSortedList (cmp : α → α → Ordering) [Std.TransCmp cmp]
+    [Std.LawfulEqCmp cmp] [DecidableEq α] : ListSet α → List α :=
+  Quotient.lift (Std.ExtTreeSet.ofList · cmp |>.toList) (by
+    intro l₁ l₂ hq
+    simp only []
+    congr 1
+    rw [Std.ExtTreeSet.ext_mem_iff]
+    intro x
+    simpa [Std.ExtTreeSet.mem_ofList, List.contains_eq_mem] using hq x
+  )
+
+end ArchSem
